verif/btrees/verif_newcursor.v
@@ -13,39 +13,22 @@ Require Import btrees_sep.
 Require Import btrees_spec.
 Require Import verif_movetofirst.
 
-Lemma upd_repeat: forall X i (a:X) b m, 0 <= i -> (Z.to_nat i < m)%nat -> m=MaxTreeDepth ->  
-    upd_Znth i (list_repeat (Z.to_nat i) a ++ list_repeat (m - Z.to_nat i) b) a =
-    (list_repeat (Z.to_nat (i+1)) a) ++ list_repeat (m - Z.to_nat (i+1)) b.
+Lemma upd_repeat: forall X i (a:X) b m, 0 <= i -> i < m -> m=MaxTreeDepth ->  
+    upd_Znth i (list_repeat (Z.to_nat i) a ++ list_repeat (Z.to_nat (m - i)) b) a =
+    (list_repeat (Z.to_nat (i+1)) a) ++ list_repeat (Z.to_nat (m - (i+1))) b.
 Proof.
-  intros. assert (Z.to_nat (i + 1) = ((Z.to_nat i) + S O)%nat).
-  rewrite Z2Nat.inj_add; auto. omega.
-  rewrite H2.
-  assert(1 <= 20 - i).
-  { rewrite H1 in H0. rewrite MTD_eq in H0.
-    replace (20%nat) with (Z.to_nat 20) in H0 by auto.
-    apply Z2Nat.inj_lt in H0. omega. auto. omega. }
+  intros.
+  pose proof I.
+  pose proof I.
+  rewrite Z2Nat.inj_add by omega.
   rewrite <- list_repeat_app.
-  rewrite upd_Znth_app2. 
-  rewrite Zlength_list_repeat by auto.
-  simpl. assert (i-i=0). omega. rewrite H4.
-  unfold upd_Znth. simpl.
-  assert ((m - (Z.to_nat i))%nat = Z.to_nat (20-i)).
-  {rewrite H1. rewrite MTD_eq. rewrite Z2Nat.inj_sub by auto. simpl. auto. }
-  assert ((m - (Z.to_nat i + 1))%nat = Z.to_nat (20-i-1)).
-  { rewrite H1. rewrite MTD_eq. rewrite Z2Nat.inj_sub by omega.
-    rewrite Z2Nat.inj_sub by auto. replace (1%nat) with (Z.to_nat 1) at 2.
-    replace (20%nat) with (Z.to_nat 20). omega. auto. auto. }
-  rewrite H5. rewrite H6. 
-  rewrite sublist_list_repeat.
-  rewrite Zlength_list_repeat. rewrite <- app_assoc. auto.
-  { rewrite H1 in H0. rewrite MTD_eq in H0. omega. }
-  omega.
-  rewrite Zlength_list_repeat. split; auto.
-  omega.
-  omega.
-  rewrite Zlength_list_repeat. split. apply Z.le_refl.
-  assert(0 <= Zlength (list_repeat (m - Z.to_nat i) b)) by apply Zlength_nonneg. omega.
-  auto.
+  replace (m-i) with (1 + (m-(i+1))) by omega.
+  rewrite Z2Nat.inj_add by omega.
+  rewrite <- list_repeat_app.
+  rewrite upd_Znth_app2 by list_solve.
+  rewrite app_ass. f_equal. 
+  autorewrite with sublist.
+  f_equal.
 Qed.
 
 Lemma body_NewCursor: semax_body Vprog Gprog f_RL_NewCursor RL_NewCursor_spec.
@@ -63,24 +46,24 @@ Proof.
     + split. unfold sizeof. simpl. rep_omega. split; auto.
     + Intros vret.
       forward_if.
-      * forward.
+      * forward. entailer!. Exists (Vint (Int.repr 0)). entailer!.
       * forward.                (* cursor->relation=relation *)
         forward.                (* cursor->level=0 *)
         unfold relation_rep. unfold r. Intros.
         forward.                  (* t'3=relation->root *)
-        simpl.
 {       forward_call(r,empty_cursor,vret,root,numrec). (* moveToFirst at level 0 *)
-        - instantiate (Frame:=[mem_mgr gv]). unfold Frame. simpl.
+        - instantiate (Frame:=[mem_mgr gv]). unfold Frame.
           unfold relation_rep. unfold r. entailer!.
           unfold cursor_rep.
-          Exists (list_repeat 20 Vundef). Exists (list_repeat 20 Vundef). unfold empty_cursor. simpl.
-          cancel.
+          do 2 Exists (list_repeat (Z.to_nat MaxTreeDepth) Vundef). 
+          unfold empty_cursor. simpl fold_right_sepcon. cancel.
         - repeat split.
           + unfold partial_cursor_correct_rel. simpl. auto.
           + unfold empty_cursor. simpl. auto.
           + auto.
         - unfold cursor_rep. Intros anc_end. Intros idx_end. unfold r.
           forward.              (* return *)
+          entailer!.
           Exists vret. entailer!. unfold cursor_rep.
           Exists anc_end. Exists idx_end. cancel. }
 Qed.
