verif/btrees/verif_splitnode_part2.v
@@ -13,6 +13,7 @@ Require Import verif_newnode.
 Require Import verif_findindex.
 Require Import index.
 Require Import verif_splitnode_part0.
+Require Import verif_splitnode_part1.
 
 
 (* Could be useful in refactoring splitnode_main_if_then_proof *)
@@ -31,7 +32,7 @@ Definition splitnode_main_if_part1 : statement :=
 
 
 
-Require Import verif_splitnode_part1.
+(*Require Import verif_splitnode_part1. *)
 
 Opaque Znth.
 
@@ -46,7 +47,7 @@ Lemma splitnode_main_if_then_proof:
   (keyrepr : val) (coprepr : val + val)
   (HEVR : entry_val_rep e = (keyrepr, coprepr))
   (k : key) (HK : keyrepr = key_repr k)
-  (INRANGE : 0 <= idx_to_Z (findRecordIndex n k) <= Z.of_nat Fanout)
+  (INRANGE : 0 <= idx_to_Z (findRecordIndex n k) <= Fanout)
   (vnewnode : val)
   (H1 : vnewnode <> nullval)
   (ent_end : list (val * (val + val)))
@@ -74,10 +75,7 @@ semax (func_tycontext f_splitnode Vprog Gprog [])
      (Val.of_bool isLeaf,
      (Val.of_bool First,
      (Vint (Int.repr 0),
-     (Vint
-        (Int.repr
-           (Z.of_nat
-              (numKeys (btnode val ptr0 le isLeaf First Last nval)))),
+     (Vint (Int.repr (numKeys (btnode val ptr0 le isLeaf First Last nval))),
      (optionally getval nullval ptr0,
       le_to_list le ++ ent_end))))) nval;
    optionally btnode_rep emp ptr0; le_iter_sepcon le;
@@ -124,28 +122,29 @@ Proof.
     { rewrite ENTRY. unfold entry_rep. entailer!. }
     rename H3 into PTRXE.
     
-    forward_for_simple_bound (Z.of_nat fri)
+    forward_for_simple_bound fri
     (EX i:Z, EX allent_end:list (val*(val+val)),
-     (PROP (length allent_end = (Fanout + 1 - Z.to_nat(i))%nat)
+     (PROP (Zlength allent_end = Fanout + 1 - i)
       LOCAL (temp _t'3 (Val.of_bool isLeaf); temp _newNode vnewnode; temp _t'2 vnewnode;
-      temp _t'27 (Val.of_bool Last); temp _tgtIdx (Vint (Int.repr (Z.of_nat fri)));
-      temp _t'1 (Vint (Int.repr (Z.of_nat fri))); temp _t'28 keyrepr;
+      temp _t'27 (Val.of_bool Last); temp _tgtIdx (Vint (Int.repr fri));
+      temp _t'1 (Vint (Int.repr fri)); temp _t'28 keyrepr;
       lvar _allEntries (tarray tentry 16) v_allEntries; temp _node nval; temp _entry pe;
       temp _isLeaf (Val.of_bool isLeaf))
       SEP (mem_mgr gv; btnode_rep nleft; btnode_rep (empty_node isLeaf false Last vnewnode);
-           data_at Tsh (tarray tentry 16) (le_to_list (nth_first_le le (Z.to_nat i))++ allent_end) v_allEntries; entry_rep e; data_at Ews tentry (keyrepr, coprepr) pe)))%assert.
-    { simpl in INRANGE. rewrite Fanout_eq in INRANGE.
-      replace (Z.of_nat 15) with 15 in INRANGE. rep_omega. simpl. auto. }
+           data_at Tsh (tarray tentry 16) (le_to_list (nth_first_le le i)++ allent_end) v_allEntries;
+           entry_rep e; data_at Ews tentry (keyrepr, coprepr) pe)))%assert.
+    { simpl in INRANGE; rep_omega. }
+    { simpl in INRANGE; rep_omega. }
     { entailer!.
       Exists (default_val (nested_field_type (tarray (Tstruct _Entry noattr) 16) [])).
-      entailer!. unfold data_at_, field_at_. simpl.  entailer!. }
+      entailer!. unfold data_at_, field_at_. simpl.
+      rewrite nth_first_sublist by omega. autorewrite with sublist. cancel. }
     {                           (* loop body *)
       rewrite unfold_btnode_rep with (n:=nleft). unfold nleft.
       Intros ent_end.
-      assert(HENTRY: exists e, nth_entry_le (Z.to_nat i) le = Some e).
+      assert(HENTRY: exists e, nth_entry_le i le = Some e).
       { apply nth_entry_le_in_range. simpl in INRANGE. rewrite Fanout_eq in INRANGE.
-        unfold n in H0. simpl in H0. rewrite H0. rewrite Fanout_eq. apply Nat2Z.inj_lt.
-        simpl. rewrite Z2Nat.id. simpl in INRANGE. omega. omega. }
+        unfold n in H0. simpl in H0. rewrite H0. rep_omega. }
       destruct HENTRY as [ei HENTRY].
       assert (HEI: exists ki vi xi, ei = keyval val ki vi xi).
       { eapply integrity_nth_leaf. eauto. rewrite LEAF. simpl. auto. eauto. }
@@ -154,15 +153,15 @@ Proof.
       { apply le_iter_sepcon_split in HENTRY. rewrite HENTRY. simpl entry_rep. entailer!. }
       rename H5 into XIPTR.
       assert(HZNTH: forall ent_end, Znth (d:=(Vundef,inl Vundef)) i (le_to_list le ++ ent_end) = entry_val_rep (keyval val ki vi xi)).
-      { intros. rewrite <- Z2Nat.id with (n:=i). apply Znth_to_list. auto. omega. }
-      assert(HIRANGE: (0 <= i < 15)).
-      { clear -INRANGE H3. simpl in INRANGE. rewrite Fanout_eq in INRANGE.
-        replace (Z.of_nat 15) with 15 in INRANGE by auto. omega. }  
+      { intros. apply Znth_to_list. auto. }
+      assert(HIRANGE: (0 <= i < Fanout)).
+      { clear -INRANGE H3. simpl in INRANGE. rep_omega. }  
       forward.                  (* t'26 = node->entries[i].key *) 
       { entailer!. rewrite HZNTH. simpl; auto. }
       rewrite HZNTH. simpl.
       Opaque Znth.
       forward.                 (* allEntries[i].key = t'26 *)
+      apply prop_right.  rep_omega.
       forward.                 (* t'25=node->entries[i]->ptr.record *)
       { rewrite HZNTH. entailer!. }
       rewrite HZNTH. simpl.
@@ -171,29 +170,22 @@ Proof.
       rename allent_end into x.
       assert(XEMP: Zlength x > 0).
       { destruct x. clear - H4 HIRANGE. simpl in H4. rewrite Fanout_eq in H4.
-        apply eq_sym in H4. apply NPeano.Nat.sub_0_le in H4. apply inj_le in H4.
-        replace (Z.of_nat (15 + 1)) with 16 in H4. rewrite Z2Nat.id in H4. rep_omega.
-        omega. simpl. auto.
-        rewrite Zlength_cons. rep_omega. }
+        apply eq_sym in H4. rewrite Zlength_nil in H4.  rep_omega. list_solve.  }
       Exists (sublist 1 (Zlength x) x). entailer!.
       { clear -H4 H3 XEMP.
         destruct x.
         - rewrite Zlength_nil in XEMP. omega.
         - rewrite sublist_1_cons. rewrite Zlength_cons. rewrite Zsuccminusone.
-          rewrite sublist_same by omega. simpl in H4. rewrite Z2Nat.inj_add by omega.
-          simpl.
-          assert((Fanout + 1 - Z.to_nat i)%nat = S(Fanout + 1 - (Z.to_nat i + 1))) by omega.
-          rewrite H in H4. inv H4. omega. }
-      assert(INUM: (Z.to_nat i <= numKeys_le le)%nat).
+          rewrite sublist_same by omega. simpl in H4. rewrite Zlength_cons in *. rep_omega. }
+      assert(INUM: i <= numKeys_le le).
       { unfold n  in H0. simpl in H0. rewrite H0. clear -INRANGE H3.
-        simpl in INRANGE. apply Nat2Z.inj_le.
-        simpl. rewrite Z2Nat.id. simpl in INRANGE. omega. omega. }
+        simpl in INRANGE. rep_omega.  }
       rewrite unfold_btnode_rep with (n:=nleft). unfold nleft. Exists ent_end. cancel.      
       rewrite upd_Znth_twice.
-      rewrite app_Znth2. rewrite le_to_list_length. rewrite numKeys_nth_first. rewrite Z2Nat.id.
+      rewrite app_Znth2. rewrite le_to_list_length. rewrite numKeys_nth_first.
       replace (i-i) with 0 by omega.
       rewrite upd_Znth_app2.
-      rewrite le_to_list_length. rewrite numKeys_nth_first. rewrite Z2Nat.id.
+      rewrite le_to_list_length. rewrite numKeys_nth_first.
       replace (i-i) with 0 by omega.
       rewrite upd_Znth_same.
       unfold upd_Znth. rewrite sublist_nil. simpl.
@@ -201,85 +193,63 @@ Proof.
       rewrite sublist_split with (lo:=0) (mid:=i) (hi:=i+1).
       erewrite sublist_len_1. rewrite <- app_nil_r with (l:=le_to_list le). rewrite HZNTH. simpl.
       rewrite app_nil_r. rewrite <- app_assoc. simpl. cancel.
-      rewrite le_to_list_length. unfold n in H0. simpl in H0. rewrite H0. rewrite Fanout_eq.
-      replace (Z.of_nat 15) with 15. omega. simpl. auto. omega.
-      rewrite le_to_list_length. unfold n in H0. simpl in H0. rewrite H0. rewrite Fanout_eq.
-      replace (Z.of_nat 15) with 15. omega. simpl. auto.
+      rewrite le_to_list_length. unfold n in H0. simpl in H0. rewrite H0. rep_omega.
+      rep_omega.
+      rewrite le_to_list_length. unfold n in H0. simpl in H0. rewrite H0. rep_omega. 
+      simpl. omega. omega.
       rewrite Zlength_app. rewrite le_to_list_length. rewrite numKeys_nth_first.
-      rewrite Z2Nat.id. omega. 
+      omega. omega. omega.
+      rewrite le_to_list_length. rewrite numKeys_nth_first. omega.
       omega. omega.
-      omega. omega.
-      rewrite le_to_list_length. rewrite numKeys_nth_first.
-      rewrite Z2Nat.id. omega.
-      omega. omega.
-      omega. omega.
-      rewrite le_to_list_length. rewrite numKeys_nth_first. rewrite Z2Nat.id. omega. omega.
-      omega.
-      rewrite Zlength_app. rewrite le_to_list_length. rewrite numKeys_nth_first. rewrite Z2Nat.id.
-      omega. omega. omega. }
+      rewrite le_to_list_length. rewrite numKeys_nth_first. omega. omega.
+      rewrite Zlength_app. rewrite le_to_list_length. rewrite numKeys_nth_first.
+      omega. omega. }
     Intros allent_end.
     forward.                    (* t'24=entry->key *)
     rewrite HK. unfold key_repr.
 
-    assert(FRIRANGE: (0 <= fri < 16)%nat).
-    { simpl in INRANGE. rewrite Fanout_eq in INRANGE. split. omega.
-      replace (Z.of_nat 15) with 15 in INRANGE.
-      apply Nat2Z.inj_lt. destruct INRANGE. eapply Z.le_lt_trans with (m:=15). rep_omega.
-      simpl. omega. simpl. auto. }
+    assert(FRIRANGE: 0 <= fri <= Fanout) by auto.
     rewrite ENTRY in HEVR. simpl in HEVR. inv HEVR.
 
     Opaque Znth.
     forward.                    (* allEntries[tgtIdx]->key = t'24 *)
+    apply prop_right; rep_omega.
     forward.                    (* t'23=entry->ptr.record *)
     forward.                    (* allEntries[tgtIdx]->ptr.record = t'23 *)
-    assert(0 <= Z.of_nat fri < Zlength (le_to_list (nth_first_le le (Z.to_nat (Z.of_nat fri))) ++ allent_end)).
+    apply prop_right; rep_omega.
+    assert(0 <= fri < Zlength (le_to_list (nth_first_le le fri) ++ allent_end)).
     { split. omega. rewrite Zlength_app. rewrite le_to_list_length.
-      rewrite numKeys_nth_first. rewrite Z2Nat.id. rewrite Zlength_correct.
-      rewrite H3. rewrite Nat2Z.id.
-      assert(Z.of_nat(Fanout + 1 - fri) > 0).
-      { rewrite Fanout_eq. simpl in INRANGE. rewrite Nat2Z.inj_sub.
-        simpl. omega. rewrite Fanout_eq in INRANGE. simpl in INRANGE. omega. }
-      omega. omega.
-      rewrite Nat2Z.id. unfold n in H0. simpl in H0. rewrite H0. rewrite Fanout_eq. omega. }
+      rewrite numKeys_nth_first.
+      rewrite H3 by rep_omega. rep_omega. change (numKeys_le le) with (numKeys n). omega. }
     rewrite upd_Znth_twice by auto. rewrite upd_Znth_same by auto.
-    deadvars!.
-    assert(FRILENGTH: Zlength (le_to_list (nth_first_le le (Z.to_nat (Z.of_nat fri)))) = Z.of_nat fri).
-    { rewrite le_to_list_length. rewrite numKeys_nth_first. rewrite Nat2Z.id. auto.
-      rewrite Nat2Z.id. unfold n in H0. simpl in H0. rewrite H0. simpl in INRANGE. omega. }
-    unfold upd_Znth. rewrite sublist_app1 by (try rep_omega; rewrite FRILENGTH; rep_omega).
-    rewrite sublist_same by (try rep_omega; rewrite FRILENGTH; rep_omega).
-    rewrite sublist_app2 by (rewrite FRILENGTH; rep_omega).
-    repeat rewrite FRILENGTH.
-    replace (Z.of_nat fri + 1 - Z.of_nat fri) with 1 by rep_omega. rewrite Zlength_app.
-    rewrite FRILENGTH.
-    replace (Z.of_nat fri + Zlength allent_end - Z.of_nat fri) with (Zlength allent_end) by rep_omega.
+    assert(FRILENGTH: Zlength (le_to_list (nth_first_le le fri)) = fri).
+    { rewrite le_to_list_length. rewrite numKeys_nth_first. auto.
+      unfold n in H0. simpl in H0. rewrite H0. simpl in INRANGE. omega. }
+    rewrite upd_Znth_app2 by omega. rewrite FRILENGTH. rewrite Z.sub_diag.
+    unfold upd_Znth. autorewrite with sublist. 
 
-    forward_for_simple_bound (Z.of_nat(Fanout)) ( EX i:Z, EX ent_end:list (val * (val+val)),
-                                                                     PROP(Z.of_nat fri <= i <= Z.of_nat Fanout; length ent_end = (Fanout - Z.to_nat(i))%nat) LOCAL(temp _newNode vnewnode; temp _tgtIdx (Vint (Int.repr (Z.of_nat fri))); lvar _allEntries (tarray tentry 16) v_allEntries; temp _node nval; temp _entry pe)
-                                                                         SEP(mem_mgr gv; btnode_rep nleft; btnode_rep (empty_node true false Last vnewnode); data_at Ews tentry (Vint (Int.repr (k_ k)), inr xe) pe; data_at Tsh (tarray tentry 16) (le_to_list (nth_first_le le (Z.to_nat (Z.of_nat fri))) ++ (Vint (Int.repr (k_ k)), inr (force_val (sem_cast_pointer xe))) :: le_to_list(suble (fri) (Z.to_nat i) le) ++ ent_end) v_allEntries; entry_rep(keyval val ke ve xe)))%assert.
+    forward_for_simple_bound Fanout
+         ( EX i:Z, EX ent_end:list (val * (val+val)),
+           PROP (fri <= i <= Fanout; Zlength ent_end = Fanout - i) 
+           LOCAL (temp _newNode vnewnode; temp _tgtIdx (Vint (Int.repr fri));
+                       lvar _allEntries (tarray tentry 16) v_allEntries; temp _node nval; temp _entry pe)
+           SEP(mem_mgr gv; btnode_rep nleft; btnode_rep (empty_node true false Last vnewnode);
+                 data_at Ews tentry (Vint (Int.repr (k_ k)), inr xe) pe;
+                 data_at Tsh (tarray tentry 16) (le_to_list (nth_first_le le fri) ++ (Vint (Int.repr (k_ k)), inr (force_val (sem_cast_pointer xe))) :: le_to_list(suble fri i le) ++ ent_end) v_allEntries; entry_rep(keyval val ke ve xe)))%assert.
 
-    { simpl in INRANGE. rewrite Fanout_eq in INRANGE.
-      replace (Z.of_nat 15) with 15 in INRANGE.
-      rewrite Fanout_eq. simpl. rep_omega. simpl. auto. }
     abbreviate_semax.
     {                           (* second loop *)
       forward.                  (* i=tgtidx *)
-      Exists (Z.of_nat(fri)). Exists ( sublist 1 (Zlength allent_end) allent_end).
+      Exists fri. Exists ( sublist 1 (Zlength allent_end) allent_end).
       entailer!.
-      simpl in INRANGE. split3; try rep_omega.
-      { clear -H3 INRANGE. destruct allent_end.
-        - simpl in H3. rewrite Nat2Z.id in H3.
-          assert((fri <= Fanout)%nat). apply Nat2Z.inj_le. omega. omega.
-        - rewrite sublist_1_cons. rewrite Zlength_cons. rewrite Zsuccminusone.
-          rewrite sublist_same; auto. simpl in H3. omega. }
-      rewrite Nat2Z.id. rewrite suble_nil. cancel. }
+      simpl in INRANGE. list_solve.
+      rewrite suble_nil. cancel. }
     {                           (* loop body *)
       rewrite unfold_btnode_rep with (n:=nleft). unfold nleft.
       rename ent_end into x.
       Intros ent_end.
-      assert(HENTRY: exists e, nth_entry_le (Z.to_nat i) le = Some e).
-      { apply nth_entry_le_in_range. simpl in H0. rewrite H0. apply Nat2Z.inj_lt.
-        rewrite Z2Nat.id. omega. omega. }
+      assert(HENTRY: exists e, nth_entry_le i le = Some e).
+      { apply nth_entry_le_in_range. simpl in H0. rewrite H0. omega. }
       destruct HENTRY as [ei HENTRY].
       assert (HEI: exists ki vi xi, ei = keyval val ki vi xi).
       { eapply integrity_nth_leaf. eauto. simpl. auto. eauto. }
@@ -289,100 +259,63 @@ Proof.
       rename H9 into XIPTR.
       rename H7 into IRANGE.
       assert(HZNTH: forall ent_end, Znth (d:=(Vundef,inl Vundef)) i (le_to_list le ++ ent_end) = entry_val_rep (keyval val ki vi xi)).
-      { intros. rewrite <- Z2Nat.id with (n:=i). apply Znth_to_list. auto. omega. }
-      assert(HIRANGE: (0 <= i < 15)).
-      { split. rep_omega. rewrite Fanout_eq in H6. simpl in H6. rep_omega. }
+      { intros. apply Znth_to_list. auto. }
+      assert(HIRANGE: (0 <= i < Fanout)) by rep_omega.
       forward.                  (* t'22=node->entries[i].key *)
       { entailer!. rewrite HZNTH. simpl; auto. }
       rewrite HZNTH. simpl.
       Opaque Znth.
       forward.                  (* allEntries[i+1].key=t'26 *)
+      apply prop_right; rep_omega.
       forward.                  (* t'21=node->entries[i].ptr.record *)
       { rewrite HZNTH. entailer!. }
       rewrite HZNTH. simpl.
       forward.                  (* allEntries[i+1]->ptr.record=t'21 *)
+      apply prop_right; rep_omega.
       entailer!.
       assert(XEMP: Zlength x > 0).
-      { destruct x. clear -H8 HIRANGE. rewrite Fanout_eq in H8.
-        apply eq_sym in H8. apply NPeano.Nat.sub_0_le in H8. apply inj_le in H8.
-        simpl in H8. rewrite Z2Nat.id in H8. rep_omega. omega.
-        rewrite Zlength_cons. rep_omega. }
+      { destruct x. clear -H8 HIRANGE. rep_omega. list_solve. }
       Exists (sublist 1 (Zlength x) x). entailer!.
-      { clear -IRANGE H8 XEMP.
-        destruct x.
-        - rewrite Zlength_nil in XEMP. omega.
-        - rewrite sublist_1_cons. rewrite Zlength_cons. rewrite Zsuccminusone.
-          rewrite sublist_same by omega. simpl in H8. rewrite Z2Nat.inj_add by omega.
-          simpl. omega. }
-      assert(INUM: (Z.to_nat i <= numKeys_le le)%nat).
-      { unfold n  in H0. simpl in H0. rewrite H0. clear -HIRANGE.
-        rewrite Fanout_eq. destruct HIRANGE. apply Z2Nat.inj_lt in H0.
-        simpl in H0. omega. auto. omega. }
+      { clear -IRANGE H8 XEMP. list_solve. }
+      assert(INUM: i <= numKeys_le le).
+      { unfold n  in H0. simpl in H0. rewrite H0. clear -HIRANGE. omega. }
       rewrite unfold_btnode_rep with (n:=nleft). unfold nleft. Exists ent_end. cancel.
-      rewrite Nat2Z.id.
       rewrite upd_Znth_twice.
       (* rewrite upd_Znth_app2. *)
       rewrite upd_Znth_same.
-      assert((upd_Znth (i + 1) (le_to_list (nth_first_le le fri) ++ (Vint (Int.repr (k_ k)), inr xe) :: le_to_list (suble (fri) ((Z.to_nat i)) le) ++ x) (key_repr ki, inr xi)) = (le_to_list (nth_first_le le fri) ++ (Vint (Int.repr (k_ k)), inr xe) :: le_to_list (suble (fri) ((Z.to_nat (i + 1))) le) ++ sublist 1 (Zlength x) x)).
+      assert((upd_Znth (i + 1) (le_to_list (nth_first_le le fri) ++ (Vint (Int.repr (k_ k)), inr xe) :: le_to_list (suble (fri) i le) ++ x) (key_repr ki, inr xi)) = (le_to_list (nth_first_le le fri) ++ (Vint (Int.repr (k_ k)), inr xe) :: le_to_list (suble fri (i + 1) le) ++ sublist 1 (Zlength x) x)).
       { rewrite upd_Znth_app2. rewrite le_to_list_length. rewrite numKeys_nth_first.
         change (?A::?B) with ([A]++B).
         rewrite upd_Znth_app2. simpl. rewrite Zlength_cons. simpl.
         rewrite upd_Znth_app2. rewrite le_to_list_length.
-        assert(i + 1 - Z.of_nat fri - 1 - Z.of_nat (numKeys_le (suble (fri) ((Z.to_nat i)) le)) = 0).
-        { rewrite numKeys_suble. simpl.
-          rewrite Nat2Z.inj_sub. rewrite Z2Nat.id. omega. omega.
-          rep_omega.
-          split. assert(fri <= Z.to_nat i)%nat.
-          rep_omega. omega.
-          simpl in H0. rewrite H0. clear -H6 HIRANGE. destruct H6.
-          rewrite Z2Nat.inj_lt in H0. rewrite Nat2Z.id in H0. omega.
-          omega. rep_omega. }
-        rewrite H17.
+        assert(i + 1 - fri - 1 - numKeys_le (suble fri i le) = 0).
+        { rewrite numKeys_suble. simpl. omega. omega. rep_omega.  }
+        rewrite H17. f_equal. f_equal.
         rewrite upd_Znth0.
-        assert(le_to_list (suble (fri) ((Z.to_nat i)) le) ++ [(key_repr ki, (inr xi):(val+val))] = le_to_list (suble (fri) ((Z.to_nat (i + 1))) le)).
-        { rewrite Z2Nat.inj_add. simpl. rewrite NPeano.Nat.add_1_r.
-          rewrite suble_increase with (e:=keyval val ki vi xi).
-          rewrite le_to_list_app. simpl. auto.
-          split. destruct IRANGE. clear -H18 HIRANGE. rewrite Nat2Z.inj_le. rewrite Z2Nat.id. auto.
-          omega.
-          simpl in H0. rewrite H0. apply Nat2Z.inj_lt.
-          rewrite Z2Nat.id. omega. omega.
-          auto. omega. omega. }
+        assert(le_to_list (suble fri i le) ++ [(key_repr ki, (inr xi):(val+val))] = le_to_list (suble fri (i + 1) le)).
+        { change (i+1) with (Z.succ i). rewrite suble_increase with (e:=keyval val ki vi xi).
+          rewrite le_to_list_app. simpl. auto. omega. auto. 
+          split. destruct IRANGE. auto. simpl in H0. rewrite H0. omega. auto. }
         rewrite <- H18. rewrite <- app_assoc. simpl. auto.
         
-        assert(Z.to_nat i < Z.to_nat (Z.of_nat Fanout))%nat. 
-        rewrite Nat2Z.id. apply Nat2Z.inj_lt. rewrite Z2Nat.id. omega. omega.
+        assert(i < Fanout) by (simpl in H0; rep_omega).
         rewrite le_to_list_length. rewrite numKeys_suble. rep_omega.
-        simpl in H0. rewrite H0. split. apply Nat2Z.inj_le. rewrite Z2Nat.id. omega. omega.
-        apply Nat2Z.inj_le. rewrite Z2Nat.id. omega. omega.
+         omega. omega.
         rewrite Zlength_cons. simpl.
         rewrite Zlength_app.
         rewrite le_to_list_length. rewrite numKeys_suble.
-        rewrite Zlength_correct. rewrite H8.
-        split. omega. rep_omega.
-        simpl in H0. rewrite H0. split. apply Nat2Z.inj_le. rewrite Z2Nat.id. omega. omega.
-        apply Nat2Z.inj_le. rewrite Z2Nat.id. omega. omega.
-        simpl in H0. rewrite H0. apply Nat2Z.inj_le. omega.
+        rewrite H8. omega. omega. omega. omega.
         rewrite Zlength_cons. rewrite Zlength_app. rewrite le_to_list_length. rewrite le_to_list_length.
-        rewrite numKeys_nth_first. rewrite numKeys_suble. split. omega.
-        rep_omega.
-        simpl in H0. rewrite H0. split. apply Nat2Z.inj_le. rewrite Z2Nat.id. omega. omega.
-        apply Nat2Z.inj_le. rewrite Z2Nat.id. omega. omega.
-        simpl in H0. rewrite H0. apply Nat2Z.inj_le. omega.
+        rewrite numKeys_nth_first. rewrite numKeys_suble. split. omega. omega. omega. omega. omega.
       }
       rewrite H17. cancel.
       rewrite Zlength_app. rewrite Zlength_cons. rewrite le_to_list_length.
       rewrite numKeys_nth_first. rewrite Zlength_app. rewrite le_to_list_length.
-      rewrite numKeys_suble. split. omega. rep_omega.
-      simpl in H0. rewrite H0. split. apply Nat2Z.inj_le. rewrite Z2Nat.id. omega. omega.
-        apply Nat2Z.inj_le. rewrite Z2Nat.id. omega. omega.
-      simpl in H0. rewrite H0. apply Nat2Z.inj_le. omega.
+      rewrite numKeys_suble. split. omega. rep_omega. omega. omega. omega.
       rewrite Zlength_app. rewrite Zlength_cons. rewrite Zlength_app.
       rewrite le_to_list_length. rewrite le_to_list_length.
-      rewrite numKeys_nth_first. rewrite numKeys_suble. split. omega. rep_omega.
-      simpl in H0. rewrite H0. split. apply Nat2Z.inj_le. rewrite Z2Nat.id. omega. omega.
-        apply Nat2Z.inj_le. rewrite Z2Nat.id. omega. omega.
-      simpl in H0. rewrite H0. apply Nat2Z.inj_le. omega.
+      rewrite numKeys_nth_first. rewrite numKeys_suble. split. omega. omega. omega. omega.
+      omega.
     } 
 
     match goal with |- semax _ _ ?c _ => change c with splitnode_main_if_part2 end.
